\chapter{Preliminaries}
% \label{chap:preliminaries}
%\addcontentsline{toc}{chapter}{Preliminaries}

This chapter provides the necessary prerequisites used throughout this project.
We begin by introducing the notation that will be employed, followed by essential definitions and
preliminary results required for formalising our arguments.

\section{Notation}

% In this section, we define the notation and symbols that will be consistently used in this work.
% Familiarity with these symbols is crucial for understanding the formal arguments and proofs presented later.

\begin{tabular}{>{\centering}m{1.8cm} m{5.8cm}}
\toprule
\textbf{Symbol} & \multicolumn{1}{c}{\textbf{Description}} \\
\midrule
$\lnot$ & Logical negation \\
$\land$ & Logical conjunction \\
$\lor$ & Logical inclusive disjunction \\
$:=$   & Definition \\
$\forall$ & Universal quantification \\
$\exists$ & Existential quantification \\
$\exists!$ & Unique existential quantification \\
$\N$ & Set of natural numbers \\
$\Z$ & Set of integer numbers \\
$\Z_n$ & Set of integers modulo $n$ \\
$\Q$ & Set of rational numbers \\
$X/Y$ & Field extension \\
$[Y:X]$ & Degree of field extension \\
$\times$ & Cartesian product \\
$[n]$ & Equivalence class of $n$ \\
$\divides$ & Divisibility relation \\
$\notdivides$ & Negation of divisibility relation \\
$\gcd$ & Greatest common divisor \\
$\zeta_n$ & Primitive $n$-th root of unity \\
\bottomrule
\end{tabular}
% \end{center}

\newpage

\section{Definitions}

In this section, each definition is articulated as clearly as possible to maximise clarity and precision.

\begin{definition-pre}[Monoid]
    \label{def:monoid}
    Let $X$ be a non-empty set.\\
    Let $\circ: X\times X \to X$ be an internal composition law on $X$. \\\\
    A \textit{monoid} is a pair $\cc{M}:= (X, \circ)$ satisfying:
    \begin{enumerate}
        \item [\textbf{(A)}] $\forall x,y,z\in X,\ (x\circ y)\circ z= x\circ (y\circ z) = x\circ y \circ z$
        \item [\textbf{(N)}] $\exists e \in X : \forall x \in X,\ x\circ e = e \circ x = x$
    \end{enumerate}
\end{definition-pre}

\begin{definition-pre}[Commutative Monoid]
    \label{def:commutative_monoid}
    Let $X$ be a non-empty set.\\
    Let $\circ: X\times X \to X$ be an internal composition law on $X$. \\\\
    A \textit{commutative monoid} is a pair $\cc{M}_c:= (X, \circ)$ satisfying:
    \begin{enumerate}
        \item [\textbf{(A)}] $\forall x,y,z\in X,\ (x\circ y)\circ z= x\circ (y\circ z) = x\circ y \circ z$
        \item [\textbf{(N)}] $\exists e \in X : \forall x \in X,\ x\circ e = e \circ x = x$
        \item [\textbf{(C)}] $\forall x,y\in X,\ x\circ y = y\circ x$
    \end{enumerate}
\end{definition-pre}

\begin{definition-pre}[GCD Monoid]
    \label{def:gcd_monoid}
    Let $X$ be a non-empty set.\\
    Let $\circ: X\times X \to X$ be an internal composition law on $X$. \\\\
    A \textit{gcd monoid} is a pair $\cc{M}_{\gcd}:= (X, \circ)$ satisfying:
    \begin{enumerate}
        \item [\textbf{(A)}] $\forall x,y,z\in X,\ (x\circ y)\circ z= x\circ (y\circ z) = x\circ y \circ z$
        \item [\textbf{(N)}] $\exists e \in X : \forall x \in X,\ x\circ e = e \circ x = x$
        \item [\textbf{(C)}] $\forall x,y\in X,\ x\circ y = y\circ x$
        \item [\textbf{(G)}] $\forall x,y\in X,\ \exists d \in X : (d\divides x) \land (d\divides y)
                             \land \left(\forall c \in X,\ c\divides x \land c\divides y \Rightarrow c\divides d\right)$
    \end{enumerate}
\end{definition-pre}

\begin{definition-pre}[Group]
    \label{def:group}
    Let $X$ be a non-empty set.\\
    Let $\circ: X\times X \to X$ be an internal composition law on $X$. \\\\
    A \textit{group} is a pair $\cc{G}:= (X, \circ)$ satisfying:
    \begin{enumerate}
        \item [\textbf{(A)}] $\forall x,y,z\in X,\ (x\circ y)\circ z= x\circ (y\circ z) = x\circ y \circ z$
        \item [\textbf{(N)}] $\exists e \in X : \forall x \in X,\ x\circ e = e \circ x = x$
        \item [\textbf{(I)}] $\forall x \in X,\ \exists x'\in X: x\circ x' = x'\circ x = e$
    \end{enumerate}
\end{definition-pre}

\begin{definition-pre}[Commutative Group]
    \label{def:commutative_group}
    Let $X$ be a non-empty set.\\
    Let $\circ: X\times X \to X$ be an internal composition law on $X$. \\\\
    A \textit{commutative group} is a pair $\cc{G}_c:= (X, \circ)$ satisfying:
    \begin{enumerate}
        \item [\textbf{(A)}] $\forall x,y,z\in X,\ (x\circ y)\circ z= x\circ (y\circ z) = x\circ y \circ z$
        \item [\textbf{(N)}] $\exists e \in X : \forall x \in X,\ x\circ e = e \circ x = x$
        \item [\textbf{(I)}] $\forall x \in X,\ \exists x'\in X: x\circ x' = x'\circ x = e$
        \item [\textbf{(C)}] $\forall x,y\in X,\ x\circ y = y\circ x$
    \end{enumerate}
\end{definition-pre}

\begin{definition-pre}[Semiring]
    \label{def:semiring}
    Let $X$ be a non-empty set. \\
    Let $+: X\times X \to X$ be an additive internal composition law on $X$. \\
    Let $\cdot: X\times X \to X$ be a multiplicative internal composition law on $X$. \\\\
    A \textit{semiring} is a triple $\cc{S}:= (X, +, \cdot)$ satisfying:
    \begin{enumerate}
        \item [\textbf{(A1)}] $\forall x,y,z\in X,\ (x+y)+z= x+(y+z) = x+y+z$
        \item [\textbf{(C1)}] $\forall x,y\in X,\ x+y = y+x$
        \item [\textbf{(N1)}] $\exists 0 \in X : \forall x \in X,\ x+0 = 0+x = x$
        \item [\textbf{(A2)}] $\forall x,y,z\in X,\ (x\cdot y)\cdot z= x\cdot(y\cdot z) = x\cdot y\cdot z$
        \item [\textbf{(N2)}] $\exists 1 \in X : \forall x \in X,\ x\cdot1 = 1\cdot x = x$
        \item [\textbf{(D1)}] $\forall x,y,z \in X,\ x\cdot(y+z)=x\cdot y+x\cdot z$
        \item [\textbf{(D2)}] $\forall x,y,z \in X,\ (x+y)\cdot z=x\cdot z+y\cdot z$
    \end{enumerate}
\end{definition-pre}
\begin{definition-pre}[Commutative Semiring]
    \label{def:commutative_semiring}
    Let $X$ be a non-empty set. \\
    Let $+: X\times X \to X$ be an additive internal composition law on $X$. \\
    Let $\cdot: X\times X \to X$ be a multiplicative internal composition law on $X$. \\\\
    A \textit{commutative semiring} is a triple $\cc{S}_c:= (X, +, \cdot)$ satisfying:
    \begin{enumerate}
        \item [\textbf{(A1)}] $\forall x,y,z\in X,\ (x+y)+z= x+(y+z) = x+y+z$
        \item [\textbf{(C1)}] $\forall x,y\in X,\ x+y = y+x$
        \item [\textbf{(N1)}] $\exists 0 \in X : \forall x \in X,\ x+0 = 0+x = x$
        \item [\textbf{(A2)}] $\forall x,y,z\in X,\ (x\cdot y)\cdot z= x\cdot(y\cdot z) = x\cdot y\cdot z$
        \item [\textbf{(C2)}] $\forall x,y\in X,\ x\cdot y = y\cdot x$
        \item [\textbf{(N2)}] $\exists 1 \in X : \forall x \in X,\ x\cdot1 = 1\cdot x = x$
        \item [\textbf{(D1)}] $\forall x,y,z \in X,\ x\cdot(y+z)=x\cdot y+x\cdot z$
        \item [\textbf{(D2)}] $\forall x,y,z \in X,\ (x+y)\cdot z=x\cdot z+y\cdot z$
    \end{enumerate}
\end{definition-pre}

\begin{definition-pre}[Ring]
    \label{def:ring}
    Let $X$ be a non-empty set. \\
    Let $+: X\times X \to X$ be an additive internal composition law on $X$. \\
    Let $\cdot: X\times X \to X$ be a multiplicative internal composition law on $X$. \\\\
    A \textit{ring} is a triple $\cc{R}:= (X, +, \cdot)$ satisfying:
    \begin{enumerate}
        \item [\textbf{(A1)}] $\forall x,y,z\in X,\ (x+y)+z= x+(y+z) = x+y+z$
        \item [\textbf{(C1)}] $\forall x,y\in X,\ x+y = y+x$
        \item [\textbf{(N1)}] $\exists 0 \in X : \forall x \in X,\ x+0 = 0+x = x$
        \item [\textbf{(I1)}] $\forall x \in X,\ \exists (-x)\in X: x+(-x) = (-x)+x = 0$
        \item [\textbf{(A2)}] $\forall x,y,z\in X,\ (x\cdot y)\cdot z= x\cdot(y\cdot z) = x\cdot y\cdot z$
        \item [\textbf{(N2)}] $\exists 1 \in X : \forall x \in X,\ x\cdot1 = 1\cdot x = x$
        \item [\textbf{(D1)}] $\forall x,y,z \in X,\ x\cdot(y+z)=x\cdot y+x\cdot z$
        \item [\textbf{(D2)}] $\forall x,y,z \in X,\ (x+y)\cdot z=x\cdot z+y\cdot z$
    \end{enumerate}
\end{definition-pre}
\begin{definition-pre}[Commutative Ring]
    \label{def:commutative_ring}
    Let $X$ be a non-empty set. \\
    Let $+: X\times X \to X$ be an additive internal composition law on $X$. \\
    Let $\cdot: X\times X \to X$ be a multiplicative internal composition law on $X$. \\\\
    A \textit{commutative ring} is a triple $\cc{R}_c:= (X, +, \cdot)$ satisfying:
    \begin{enumerate}
        \item [\textbf{(A1)}] $\forall x,y,z\in X,\ (x+y)+z= x+(y+z) = x+y+z$
        \item [\textbf{(C1)}] $\forall x,y\in X,\ x+y = y+x$
        \item [\textbf{(N1)}] $\exists 0 \in X : \forall x \in X,\ x+0 = 0+x = x$
        \item [\textbf{(I1)}] $\forall x \in X,\ \exists (-x)\in X: x+(-x) = (-x)+x = 0$
        \item [\textbf{(A2)}] $\forall x,y,z\in X,\ (x\cdot y)\cdot z= x\cdot(y\cdot z) = x\cdot y\cdot z$
        \item [\textbf{(C2)}] $\forall x,y\in X,\ x\cdot y = y\cdot x$
        \item [\textbf{(N2)}] $\exists 1 \in X : \forall x \in X,\ x\cdot1 = 1\cdot x = x$
        \item [\textbf{(D1)}] $\forall x,y,z \in X,\ x\cdot(y+z)=x\cdot y+x\cdot z$
        \item [\textbf{(D2)}] $\forall x,y,z \in X,\ (x+y)\cdot z=x\cdot z+y\cdot z$
    \end{enumerate}
\end{definition-pre}

\begin{definition-pre}[Left Ideal]
    \label{def:left_ideal}
    Let $(X, +, \cdot)$ be a ring. \\\\
    A \textit{left ideal} is a subset $I \subseteq X$ satisfying:
    \begin{enumerate}
        \item [\textbf{(SG)}] $(I, +)$ is a subgroup of $(X, +)$
        \item [\textbf{(L)}] $\forall i\in I,\ \forall x\in X,\ x\cdot i\in I$
    \end{enumerate}
\end{definition-pre}

\begin{definition-pre}[Right Ideal]
    \label{def:right_ideal}
    Let $(X, +, \cdot)$ be a ring. \\\\
    A \textit{right ideal} is a subset $I \subseteq X$ satisfying:
    \begin{enumerate}
        \item [\textbf{(SG)}] $(I, +)$ is a subgroup of $(X, +)$
        \item [\textbf{(R)}] $\forall i\in I,\ \forall x\in X,\ i\cdot x\in I$
    \end{enumerate}
\end{definition-pre}

\begin{definition-pre}[Ideal]
    \label{def:ideal}
    Let $(X, +, \cdot)$ be a ring. \\\\
    An \textit{ideal} or \textit{two-sided ideal} is a subset $I \subseteq X$ satisfying:
    \begin{enumerate}
        \item [\textbf{(SG)}] $(I, +)$ is a subgroup of $(X, +)$
        \item [\textbf{(L)}] $\forall i\in I,\ \forall x\in X,\ x\cdot i\in I$
        \item [\textbf{(R)}] $\forall i\in I,\ \forall x\in X,\ i\cdot x\in I$
    \end{enumerate}
\end{definition-pre}

\begin{definition-pre}[Domain]
    \label{def:domain}
    Let $X$ be a non-empty set. \\
    Let $+: X\times X \to X$ be an additive internal composition law on $X$. \\
    Let $\cdot: X\times X \to X$ be a multiplicative internal composition law on $X$. \\\\
    A \textit{domain} is a triple $\cc{D}:= (X, +, \cdot)$ satisfying:
    \begin{enumerate}
        \item [\textbf{(A1)}] $\forall x,y,z\in X,\ (x+y)+z= x+(y+z) = x+y+z$
        \item [\textbf{(C1)}] $\forall x,y\in X,\ x+y = y+x$
        \item [\textbf{(N1)}] $\exists 0 \in X : \forall x \in X,\ x+0 = 0+x = x$
        \item [\textbf{(I1)}] $\forall x \in X,\ \exists (-x)\in X: x+(-x) = (-x)+x = 0$
        \item [\textbf{(A2)}] $\forall x,y,z\in X,\ (x\cdot y)\cdot z= x\cdot(y\cdot z) = x\cdot y\cdot z$
        \item [\textbf{(N2)}] $\exists 1 \in X : \forall x \in X,\ x\cdot1 = 1\cdot x = x$
        \item [\textbf{(D1)}] $\forall x,y,z \in X,\ x\cdot(y+z)=x\cdot y+x\cdot z$
        \item [\textbf{(D2)}] $\forall x,y,z \in X,\ (x+y)\cdot z=x\cdot z+y\cdot z$
        \item [\textbf{(Z2)}] $\forall x,y \in X,\ x\cdot y = 0 \Rightarrow x=0 \lor y=0$
    \end{enumerate}
\end{definition-pre}

\begin{definition-pre}[Commutative Domain]
    \label{def:commutative_domain}
    Let $X$ be a non-empty set. \\
    Let $+: X\times X \to X$ be an additive internal composition law on $X$. \\
    Let $\cdot: X\times X \to X$ be a multiplicative internal composition law on $X$. \\\\
    A \textit{commutative} or \textit{integral domain} is a triple $\cc{D}_c:= (X, +, \cdot)$ satisfying:
    \begin{enumerate}
        \item [\textbf{(A1)}] $\forall x,y,z\in X,\ (x+y)+z= x+(y+z) = x+y+z$
        \item [\textbf{(C1)}] $\forall x,y\in X,\ x+y = y+x$
        \item [\textbf{(N1)}] $\exists 0 \in X : \forall x \in X,\ x+0 = 0+x = x$
        \item [\textbf{(I1)}] $\forall x \in X,\ \exists (-x)\in X: x+(-x) = (-x)+x = 0$
        \item [\textbf{(A2)}] $\forall x,y,z\in X,\ (x\cdot y)\cdot z= x\cdot(y\cdot z) = x\cdot y\cdot z$
        \item [\textbf{(C2)}] $\forall x,y\in X,\ x\cdot y = y\cdot x$
        \item [\textbf{(N2)}] $\exists 1 \in X : \forall x \in X,\ x\cdot1 = 1\cdot x = x$
        \item [\textbf{(D1)}] $\forall x,y,z \in X,\ x\cdot(y+z)=x\cdot y+x\cdot z$
        \item [\textbf{(D2)}] $\forall x,y,z \in X,\ (x+y)\cdot z=x\cdot z+y\cdot z$
        \item [\textbf{(Z2)}] $\forall x,y \in X,\ x\cdot y = 0 \Rightarrow x=0 \lor y=0$
    \end{enumerate}
\end{definition-pre}

\begin{definition-pre}[Field]
    \label{def:field}
    Let $X$ be a non-empty set. \\
    Let $+: X\times X \to X$ be an additive internal composition law on $X$. \\
    Let $\cdot: X\times X \to X$ be a multiplicative internal composition law on $X$. \\\\
    A \textit{field} is a triple $\bb{F}:= (X, +, \cdot)$ satisfying:
    \begin{enumerate}
        \item [\textbf{(A1)}] $\forall x,y,z\in X,\ (x+y)+z= x+(y+z) = x+y+z$
        \item [\textbf{(C1)}] $\forall x,y\in X,\ x+y = y+x$
        \item [\textbf{(N1)}] $\exists 0 \in X : \forall x \in X,\ x+0 = 0+x = x$
        \item [\textbf{(I1)}] $\forall x \in X,\ \exists (-x)\in X: x+(-x) = (-x)+x = 0$
        \item [\textbf{(A2)}] $\forall x,y,z\in X,\ (x\cdot y)\cdot z= x\cdot(y\cdot z) = x\cdot y\cdot z$
        \item [\textbf{(N2)}] $\exists 1 \in X : \forall x \in X,\ x\cdot1 = 1\cdot x = x$
        \item [\textbf{(I2)}] $\forall x \in X,\ \exists x^{-1}\in X: x\cdot x^{-1} = x^{-1}\cdot x = 1$
        \item [\textbf{(D1)}] $\forall x,y,z \in X,\ x\cdot(y+z)=x\cdot y+x\cdot z$
        \item [\textbf{(D2)}] $\forall x,y,z \in X,\ (x+y)\cdot z=x\cdot z+y\cdot z$
    \end{enumerate}
\end{definition-pre}

\begin{definition-pre}[Commutative Field]
    \label{def:commutative_field}
    Let $X$ be a non-empty set. \\
    Let $+: X\times X \to X$ be an additive internal composition law on $X$. \\
    Let $\cdot: X\times X \to X$ be a multiplicative internal composition law on $X$. \\\\
    A \textit{commutative field} is a triple $\bb{F}_c:= (X, +, \cdot)$ satisfying:
    \begin{enumerate}
        \item [\textbf{(A1)}] $\forall x,y,z\in X,\ (x+y)+z= x+(y+z) = x+y+z$
        \item [\textbf{(C1)}] $\forall x,y\in X,\ x+y = y+x$
        \item [\textbf{(N1)}] $\exists 0 \in X : \forall x \in X,\ x+0 = 0+x = x$
        \item [\textbf{(I1)}] $\forall x \in X,\ \exists (-x)\in X: x+(-x) = (-x)+x = 0$
        \item [\textbf{(A2)}] $\forall x,y,z\in X,\ (x\cdot y)\cdot z= x\cdot(y\cdot z) = x\cdot y\cdot z$
        \item [\textbf{(C2)}] $\forall x,y\in X,\ x\cdot y = y\cdot x$
        \item [\textbf{(N2)}] $\exists 1 \in X : \forall x \in X,\ x\cdot1 = 1\cdot x = x$
        \item [\textbf{(I2)}] $\forall x \in X,\ \exists x^{-1}\in X: x\cdot x^{-1} = x^{-1}\cdot x = 1$
        \item [\textbf{(D1)}] $\forall x,y,z \in X,\ x\cdot(y+z)=x\cdot y+x\cdot z$
        \item [\textbf{(D2)}] $\forall x,y,z \in X,\ (x+y)\cdot z=x\cdot z+y\cdot z$
    \end{enumerate}
\end{definition-pre}

\begin{definition-pre}[Fundamental System of Field]
	\label{def:fundamental_system}
    Let $(X, +, \cdot)$ be a field endowed with a topology $\mathcal{T}$. \\
    Let $I \subseteq \N$ be an index set. \\\\
    A \textit{fundamental system} of $X$ is a collection \( \mathcal{U} = \{ U_i \}_{i \in I} \) of open sets in \( X \) such that:
	\begin{enumerate}
		\item $\forall i \in I,\ 0 \in U_i$.
		\item $\forall V \ni 0,\ \exists i \in I : U_i \subseteq V$.
	\end{enumerate}
\end{definition-pre}

\begin{definition-pre}[Vector Space]
    \label{def:vector_space}
    Let $X$ be a non-empty set. \\
    Let $(\K,+,\cdot)$ be a field. \\
    Let $+: X\times X \to X$ be an additive internal composition law on $X$. \\
    Let $\cdot: \K\times X \to X$ be a multiplicative external composition law on $X$. \\\\
    A \K-\textbf{vector space} or \K-\textbf{linear space} is a triple $\cc{V}:= (X, +, \cdot)_{\K}$ satisfying:
    \begin{enumerate}
        \item [\textbf{(A)}] $\forall x,y,z\in X,\ (x+y)+z= x+(y+z) = x+y+z$
        \item [\textbf{(C)}] $\forall x,y\in X,\ x+y = y+x$
        \item [\textbf{(N)}] $\exists 0 \in X : \forall x \in X,\ x+0 = 0+x = x$
        \item [\textbf{(I)}] $\forall x \in X,\ \exists (-x)\in X: x+(-x) = (-x)+x = 0$
        \item [\textbf{(P)}] $\forall x \in X,\ \forall k,\ell \in \K,\ k\cdot_X(\ell\cdot_X x)= (k\cdot_{\K}\ell)\cdot_X x$
        \item [\textbf{(U)}] $\exists 1 \in \K : \forall x \in X,\ 1\cdot x = x$
        \item [\textbf{(D1)}] $\forall x,y \in X,\ \forall k\in \K,\ k\cdot(x+_Xy)=k\cdot x+_Xk\cdot y$
        \item [\textbf{(D2)}] $\forall k,\ell \in \K,\ \forall x\in X,\ (k+_\K\ell)\cdot x=k\cdot x+_X\ell\cdot x$
    \end{enumerate}
\end{definition-pre}

From now on, we shall employ the notation $X$ in place of the more explicit $(X, +, \cdot)$ to denote a field,
commutative ring, domain, or similar algebraic structures when the context unambiguously implies the operations involved.

\begin{definition-pre}[Field Extension]
    \label{def:field_extension}
    Let $(X, +, \cdot)$ be a field. \\
    Let $(Y, +, \cdot)$ be a field such that $Y \subseteq X$. \\\\
    A \textit{field extension} is the pair $X/Y$ such that the operations of $Y$
    are those of $X$ restricted to $Y$.
\end{definition-pre}

\begin{definition-pre}[Degree of Field Extension]
    \label{def:degree_field_extension}
    Let $(X, +, \cdot)$ be a field. \\
    Let $(Y, +, \cdot)$ be a field such that $Y \subseteq X$. \\
    Let $X/Y$ be a field extension. \\\\
    The \textit{degree} of $X/Y$, denoted as $[Y:X]$, is the dimension of $X$ as a vector space over $Y$.
\end{definition-pre}

\begin{definition-pre}[Algebraic Field Extension]
    \label{def:algebraic_field_extension}
    Let $(X, +, \cdot)$ be a field. \\
    Let $(Y, +, \cdot)$ be a field such that $Y \subseteq X$. \\\\
    An \textit{algebraic field extension} is the field extension $X/Y$ such that its degree $[Y:X]$
    is finite.
\end{definition-pre}

\begin{definition-pre}[Extension Field]
    \label{def:extension_field}
    Let $(X, +, \cdot)$ be a field. \\
    Let $(Y, +, \cdot)$ be a field such that $Y \subseteq X$. \\
    Let $X/Y$ be a field extension. \\\\
    The field $X$ is said to be an \textit{extension field} of $Y$.
\end{definition-pre}

\begin{definition-pre}[Subfield]
    \label{def:subfield}
    Let $(X, +, \cdot)$ be a field. \\
    Let $(Y, +, \cdot)$ be a field such that $Y \subseteq X$. \\
    Let $X/Y$ be a field extension. \\\\
    The field $Y$ is said to be a \textit{subfield} of $X$.
\end{definition-pre}

\begin{definition-pre}[Number Field]
    \label{def:number_field}
    Let $(X, +, \cdot)$ be a field. \\
    Let $(\Q, +, \cdot)$ be the field of rational numbers such that $\Q \subseteq X$. \\
    Let $X/\Q$ be an algebraic field extension. \\\\
    The extension field $X$ is said to be a \textit{number field} or an \textit{algebraic number field}.
\end{definition-pre}

\begin{definition-pre}[Root of Unity]
    \label{def:root_of_unity}
    Let $n \in \N_{+}$. \\\\
    A \textit{$n$-th root of unity} is an element $\zeta \in \C$ such that  $\zeta^n = 1$.
\end{definition-pre}

\begin{definition-pre}[Primitive Root of Unity]
    \label{def:primitive_root_of_unity}
    Let $n \in \N_{+}$. \\\\
    A \textit{primitive $n$-th root of unity} is an element $\zeta \in \C$ satisfying:
    \begin{enumerate}
        \item $\zeta^n = 1$.
        \item $\forall k \in \N_{+},\ k < n \implies \zeta^k \neq 1$.
    \end{enumerate}
\end{definition-pre}

\begin{definition-pre}[Cyclotomic Polynomial]
    \label{def:cyclotomic_polynomial}
    Let $n \in \N_{+}$. \\
    Let $\zeta \in \C$ be a primitive $n$-th root of unity. \\\\
    The \textit{$n$-th cyclotomic polynomial} is the unique monic polynomial with integer coefficients whose roots are the primitive $n$-th roots of unity:
    $$ \Phi_n(x) = \prod_{\substack{1 \leq k \leq n \\ \gcd(k, n) = 1}} \left( x - \zeta^k \right)$$
\end{definition-pre}

\begin{definition-pre}[Cyclotomic Extension Field]
    \label{def:cyclotomic_extension_field}
    Let $n \in \N_{+}$. \\
    Let $\zeta_n \in \C$ be a primitive $n$-th root of unity. \\
    Let $X$ be a field. \\\\
    The \textit{$n$-th cyclotomic extension field} or \textit{$n$-th cyclotomic field} is a field $X(\zeta_n)$ obtained by adjoining $\zeta_n$ to $X$.
\end{definition-pre}

\section{Results}

In this section, we state some preliminary results that are crucial for the development of our formal proofs.

\begin{theorem}
    \label{thm:zeta_sub_one_prime1}
    \lean{IsPrimitiveRoot.zeta_sub_one_prime'}
    \leanok
    Let $p \in \N$ be prime. \\\\
    If $\zeta_p$ is a primitive $p$-th root of unity, then $\zeta_p - 1$ is prime.
\end{theorem}
\begin{proof}
    \leanok
    This has already been formalised and included in \href{https://pitmonticone.github.io/FLT3/docs/FLT3/Mathlib/NumberTheory/Cyclotomic/Rat.html#IsPrimitiveRoot.zeta_sub_one_prime'}{Mathlib}.
\end{proof}

\begin{lemma}
    \label{lmm:fermatLastTheoremWith_of_fermatLastTheoremWith_coprime}
    \lean{fermatLastTheoremWith_of_fermatLastTheoremWith_coprime}
    \leanok
    Let $R$ be a commutative semiring, domain and normalised $\gcd$ monoid.\\% ASK EXPERTS
    Let $a, b, c \in R$. \\
    Let $n \in \N$. \\\\
    Then, to prove Fermat's Last Theorem for exponent $n$ in $R$,
    one can assume, without loss of generality, that $\gcd(a,b,c)=1$.
  \end{lemma}
  \begin{proof}
    \leanok
    This has already been formalised and included in \href{https://pitmonticone.github.io/FLT3/docs/FLT3/Mathlib/NumberTheory/FLT/Basic.html#fermatLastTheoremWith_of_fermatLastTheoremWith_coprime}{Mathlib}.
  \end{proof}

  \begin{lemma}
    \label{lmm:cube_of_castHom_ne_zero}
    \lean{cube_of_castHom_ne_zero}
    \leanok
    Let $\Z_9$ be the ring of integers modulo $9$. \\
    Let $\Z_3$ be the ring of integers modulo $3$. \\
    Let $n \in \Z_9$. \\
    Let $\phi : \Z_9 \to \Z_3$ be the canonical ring homomorphism. \\
    Let $\phi(n) \neq 0$. \\ \\
    Then $n^3=1 \lor n^3=8$.
  \end{lemma}
  \begin{proof}
    \leanok
    This has already been formalised and included in \href{https://pitmonticone.github.io/FLT3/docs/FLT3/Mathlib/NumberTheory/FLT/Three.html#cube_of_castHom_ne_zero}{Mathlib}.
  \end{proof}